theories/SLFWP.v
@@ -1,0 +1,13 @@
+
+
+forward proof 
+- with let
+- lets
+- subst all pb
+
+reasoning on calls
+- with = 2*x (app vs apps)
+- with y st P x y
+
+recursion
+- call that does not fit coq
